@prefix : <http://example.org/fho/> .
@prefix dc: <http://purl.org/dc/elements/1.1/> .
@prefix ex: <http://example.org/> .
@prefix kb: <http://example.org/fho/kb/> .
@prefix mto: <http://purl.org/ontology/mto/> .
@prefix ns1: <http://www.w3.org/2003/11/swrl#> .
@prefix owl: <http://www.w3.org/2002/07/owl#> .
@prefix rdf: <http://www.w3.org/1999/02/22-rdf-syntax-ns#> .
@prefix xml: <http://www.w3.org/XML/1998/namespace> .
@prefix xsd: <http://www.w3.org/2001/XMLSchema#> .
@prefix rdfs: <http://www.w3.org/2000/01/rdf-schema#> .
@prefix chord: <http://purl.org/ontology/chord/> .
@prefix mto-kb: <http://purl.org/ontology/mto/kb/> .
@base <http://example.org/fho/> .

<http://example.org/fho/> rdf:type owl:Ontology ;
                           owl:imports <http://purl.org/ontology/mto/0.9> .

#################################################################
#    Annotation properties
#################################################################

###  http://purl.org/ontology/chord/interval
chord:interval rdf:type owl:AnnotationProperty .


###  http://swrl.stanford.edu/ontologies/3.3/swrla.owl#isRuleEnabled
<http://swrl.stanford.edu/ontologies/3.3/swrla.owl#isRuleEnabled> rdf:type owl:AnnotationProperty .


###  http://www.w3.org/2000/01/rdf-schema#comment
rdfs:comment rdf:type owl:AnnotationProperty .


###  http://www.w3.org/2000/01/rdf-schema#label
rdfs:label rdf:type owl:AnnotationProperty .


#################################################################
#    Datatypes
#################################################################

###  http://www.w3.org/1999/02/22-rdf-syntax-ns#PlainLiteral
rdf:PlainLiteral rdf:type rdfs:Datatype .


###  http://www.w3.org/2001/XMLSchema#boolean
xsd:boolean rdf:type rdfs:Datatype .


###  http://www.w3.org/2001/XMLSchema#string
xsd:string rdf:type rdfs:Datatype .


#################################################################
#    Object Properties
#################################################################

###  http://purl.org/ontology/mto/hasRootNote
mto:hasRootNote rdf:type owl:ObjectProperty .


#################################################################
#    Classes
#################################################################

###  http://example.org/fho/AeolianMode
:AeolianMode rdf:type owl:Class ;
             owl:equivalentClass mto:NaturalMinorScale ;
             rdfs:subClassOf :Mode ;
             rdfs:comment "Mode formed starting from the sixth degree of a major scale."^^xsd:string ;
             rdfs:label "Aeolian Mode"^^xsd:string .


###  http://example.org/fho/DorianMode
:DorianMode rdf:type owl:Class ;
            rdfs:subClassOf :Mode ;
            rdfs:comment "Mode formed starting from the second degree of a major scale."^^xsd:string ;
            rdfs:label "Dorian Mode"^^xsd:string .


###  http://example.org/fho/IonianMode
:IonianMode rdf:type owl:Class ;
            owl:equivalentClass mto:MajorScale ;
            rdfs:subClassOf :Mode ;
            rdfs:comment "Mode formed starting from the first degree of a major scale."^^xsd:string ;
            rdfs:label "Ionian Mode"^^xsd:string .


###  http://example.org/fho/LocrianMode
:LocrianMode rdf:type owl:Class ;
             rdfs:subClassOf :Mode ;
             rdfs:comment "Mode formed starting from the seventh degree of a major scale."^^xsd:string ;
             rdfs:label "Locrian Mode"^^xsd:string .


###  http://example.org/fho/LydianMode
:LydianMode rdf:type owl:Class ;
            rdfs:subClassOf :Mode ;
            rdfs:comment "Mode formed starting from the fourth degree of a major scale."^^xsd:string ;
            rdfs:label "Lydian Mode"^^xsd:string .


###  http://example.org/fho/MixolydianMode
:MixolydianMode rdf:type owl:Class ;
                rdfs:subClassOf :Mode ;
                rdfs:comment "Mode formed starting from the fifth degree of a major scale."^^xsd:string ;
                rdfs:label "Mixolydian Mode"^^xsd:string .


###  http://example.org/fho/Mode
:Mode rdf:type owl:Class ;
      rdfs:subClassOf mto:HeptatonicScale ;
      rdfs:comment "A type of scale coupled with a set of characteristic melodic and harmonic behaviors defined by the root note of the scale." ;
      rdfs:label "Mode"^^xsd:string .


###  http://example.org/fho/PhrygianMode
:PhrygianMode rdf:type owl:Class ;
              rdfs:subClassOf :Mode ;
              rdfs:comment "Mode formed starting from the third degree of a major scale."^^xsd:string ;
              rdfs:label "Phrygian Mode"^^xsd:string .


###  http://purl.org/ontology/mto/MajorScale

###  http://purl.org/ontology/mto/NaturalMinorScale

#################################################################
#    Rules
#################################################################

<urn:swrl:var#x> rdf:type ns1:Variable .

[ rdf:type ns1:Imp ;
   ns1:body [ rdf:type ns1:AtomList ;
              rdf:first [ rdf:type ns1:ClassAtom ;
                          ns1:classPredicate :Mode ;
                          ns1:argument1 <urn:swrl:var#x>
                        ] ;
              rdf:rest rdf:nil
            ] ;
   ns1:head [ rdf:type ns1:AtomList ;
              rdf:first [ rdf:type ns1:ClassAtom ;
                          ns1:classPredicate :Mode ;
                          ns1:argument1 <urn:swrl:var#x>
                        ] ;
              rdf:rest rdf:nil
            ]
 ] .

###  Generated by the OWL API (version 4.5.9.2019-02-01T07:24:44Z) https://github.com/owlcs/owlapi
