@prefix : <http://example.org/fho/> .
@prefix kb: <http://example.org/fho/kb/> .
@prefix mto: <http://purl.org/ontology/mto/> .
@prefix owl: <http://www.w3.org/2002/07/owl#> .
@prefix rdf: <http://www.w3.org/1999/02/22-rdf-syntax-ns#> .
@prefix xml: <http://www.w3.org/XML/1998/namespace> .
@prefix xsd: <http://www.w3.org/2001/XMLSchema#> .
@prefix rdfs: <http://www.w3.org/2000/01/rdf-schema#> .
@prefix chord: <http://purl.org/ontology/chord/> .
@prefix mto-kb: <http://purl.org/ontology/mto/kb/> .
@base <http://example.org/fho/> .

<http://example.org/fho/> rdf:type owl:Ontology ;
                           owl:imports <http://purl.org/ontology/mto/0.9> .

#################################################################
#    Annotation properties
#################################################################

###  http://www.w3.org/2000/01/rdf-schema#comment
rdfs:comment rdf:type owl:AnnotationProperty .


###  http://www.w3.org/2000/01/rdf-schema#label
rdfs:label rdf:type owl:AnnotationProperty .


#################################################################
#    Datatypes
#################################################################

###  http://www.w3.org/1999/02/22-rdf-syntax-ns#PlainLiteral
rdf:PlainLiteral rdf:type rdfs:Datatype .


###  http://www.w3.org/2001/XMLSchema#string
xsd:string rdf:type rdfs:Datatype .


#################################################################
#    Object Properties
#################################################################

###  http://example.org/fho/hasAeolianDominantChord
:hasAeolianDominantChord rdf:type owl:ObjectProperty ;
                         rdfs:subPropertyOf :hasDominantChord ;
                         rdfs:domain :AeolianModeScale ;
                         rdfs:range mto:MinorTriad ;
                         rdfs:comment "Property to assign the chord with dominant degree to a Aeolian mode scale"^^xsd:string ;
                         rdfs:label "has dominant chord in Aeolian mode" .


###  http://example.org/fho/hasAeolianLeadingtoneChord
:hasAeolianLeadingtoneChord rdf:type owl:ObjectProperty ;
                            rdfs:subPropertyOf :hasLeadingtoneChord ;
                            rdfs:domain :AeolianModeScale ;
                            rdfs:range mto:MajorTriad ;
                            rdfs:comment "Property to assign the chord with leadingtone degree to a Aeolian mode scale"^^xsd:string ;
                            rdfs:label "has leadingtone chord in Aeolian mode" .


###  http://example.org/fho/hasAeolianMediantChord
:hasAeolianMediantChord rdf:type owl:ObjectProperty ;
                        rdfs:subPropertyOf :hasMediantChord ;
                        rdfs:domain :AeolianModeScale ;
                        rdfs:range mto:MajorTriad ;
                        rdfs:comment "Property to assign the chord with mediant degree to a Aeolian mode scale"^^xsd:string ;
                        rdfs:label "has mediant chord in Aeolian mode" .


###  http://example.org/fho/hasAeolianSubdominantChord
:hasAeolianSubdominantChord rdf:type owl:ObjectProperty ;
                            rdfs:subPropertyOf :hasSubdominantChord ;
                            rdfs:domain :AeolianModeScale ;
                            rdfs:range mto:MinorTriad ;
                            rdfs:comment "Property to assign the chord with subdominant degree to a Aeolian mode scale"^^xsd:string ;
                            rdfs:label "has subdominant chord in Aeolian mode" .


###  http://example.org/fho/hasAeolianSubmediantChord
:hasAeolianSubmediantChord rdf:type owl:ObjectProperty ;
                           rdfs:subPropertyOf :hasSubmediantChord ;
                           rdfs:domain :AeolianModeScale ;
                           rdfs:range mto:MajorTriad ;
                           rdfs:comment "Property to assign the chord with submediant degree to a Aeolian mode scale"^^xsd:string ;
                           rdfs:label "has submediant chord in Aeolian mode" .


###  http://example.org/fho/hasAeolianSupertonicChord
:hasAeolianSupertonicChord rdf:type owl:ObjectProperty ;
                           rdfs:subPropertyOf :hasSupertonicChord ;
                           rdfs:domain :AeolianModeScale ;
                           rdfs:range mto:DiminishedTriad ;
                           rdfs:comment "Property to assign the chord with supertonic degree to a Aeolian mode scale"^^xsd:string ;
                           rdfs:label "has supertonic chord in Aeolian mode" .


###  http://example.org/fho/hasAeolianTonicChord
:hasAeolianTonicChord rdf:type owl:ObjectProperty ;
                      rdfs:subPropertyOf :hasTonicChord ;
                      rdfs:domain :AeolianModeScale ;
                      rdfs:range mto:MinorTriad ;
                      rdfs:comment "Property to assign the chord with tonic degree to a Aeolian mode scale"^^xsd:string ;
                      rdfs:label "has tonic chord in Aeolian mode" .


###  http://example.org/fho/hasChord
:hasChord rdf:type owl:ObjectProperty ;
          rdfs:domain mto:Scale ;
          rdfs:range mto:Note .


###  http://example.org/fho/hasDominantChord
:hasDominantChord rdf:type owl:ObjectProperty ;
                  rdfs:subPropertyOf :hasChord ;
                  rdfs:domain mto:Scale ;
                  rdfs:range mto:Chord ;
                  owl:propertyChainAxiom ( :hasDominantNote
                                           [ owl:inverseOf chord:root
                                           ]
                                         ) ;
                  rdfs:comment "Property to assign the chord with dominant degree to a scale"^^xsd:string ;
                  rdfs:label "has dominant chord" .


###  http://example.org/fho/hasDominantNote
:hasDominantNote rdf:type owl:ObjectProperty ;
                 rdfs:subPropertyOf mto:hasNote ;
                 rdfs:domain mto:Scale ;
                 rdfs:range mto:Note ;
                 rdfs:comment "Property to assign the note with dominant degree to a scale"^^xsd:string ;
                 rdfs:label "has dominant note" .


###  http://example.org/fho/hasDorianDominantChord
:hasDorianDominantChord rdf:type owl:ObjectProperty ;
                        rdfs:subPropertyOf :hasDominantChord ;
                        rdfs:domain :DorianModeScale ;
                        rdfs:range mto:MinorTriad ;
                        rdfs:comment "Property to assign the chord with dominant degree to a Dorian mode scale"^^xsd:string ;
                        rdfs:label "has dominant chord in Dorian mode" .


###  http://example.org/fho/hasDorianLeadingtoneChord
:hasDorianLeadingtoneChord rdf:type owl:ObjectProperty ;
                           rdfs:subPropertyOf :hasLeadingtoneChord ;
                           rdfs:domain :DorianModeScale ;
                           rdfs:range mto:MajorTriad ;
                           rdfs:comment "Property to assign the chord with leadingtone degree to a Dorian mode scale"^^xsd:string ;
                           rdfs:label "has leadingtone chord in Dorian mode" .


###  http://example.org/fho/hasDorianMediantChord
:hasDorianMediantChord rdf:type owl:ObjectProperty ;
                       rdfs:subPropertyOf :hasMediantChord ;
                       rdfs:domain :DorianModeScale ;
                       rdfs:range mto:MajorTriad ;
                       rdfs:comment "Property to assign the chord with mediant degree to a Dorian mode scale"^^xsd:string ;
                       rdfs:label "has mediant chord in Dorian mode" .


###  http://example.org/fho/hasDorianSubdominantChord
:hasDorianSubdominantChord rdf:type owl:ObjectProperty ;
                           rdfs:subPropertyOf :hasSubdominantChord ;
                           rdfs:domain :DorianModeScale ;
                           rdfs:range mto:MajorTriad ;
                           rdfs:comment "Property to assign the chord with subdominant degree to a Dorian mode scale"^^xsd:string ;
                           rdfs:label "has subdominant chord in Dorian mode" .


###  http://example.org/fho/hasDorianSubmediantChord
:hasDorianSubmediantChord rdf:type owl:ObjectProperty ;
                          rdfs:subPropertyOf :hasSubmediantChord ;
                          rdfs:domain :DorianModeScale ;
                          rdfs:range mto:DiminishedTriad ;
                          rdfs:comment "Property to assign the chord with submediant degree to a Dorian mode scale"^^xsd:string ;
                          rdfs:label "has submediant chord in Dorian mode" .


###  http://example.org/fho/hasDorianSupertonicChord
:hasDorianSupertonicChord rdf:type owl:ObjectProperty ;
                          rdfs:subPropertyOf :hasSupertonicChord ;
                          rdfs:domain :DorianModeScale ;
                          rdfs:range mto:MinorTriad ;
                          rdfs:comment "Property to assign the chord with supertonic degree to a Dorian mode scale"^^xsd:string ;
                          rdfs:label "has supertonic chord in Dorian mode" .


###  http://example.org/fho/hasDorianTonicChord
:hasDorianTonicChord rdf:type owl:ObjectProperty ;
                     rdfs:subPropertyOf :hasTonicChord ;
                     rdfs:domain :DorianModeScale ;
                     rdfs:range mto:MinorTriad ;
                     rdfs:comment "Property to assign the chord with tonic degree to a Dorian mode scale"^^xsd:string ;
                     rdfs:label "has tonic chord in Dorian mode" .


###  http://example.org/fho/hasIonianDominantChord
:hasIonianDominantChord rdf:type owl:ObjectProperty ;
                        rdfs:subPropertyOf :hasDominantChord ;
                        rdfs:domain :IonianModeScale ;
                        rdfs:range mto:MajorTriad ;
                        rdfs:comment "Property to assign the chord with dominant degree to a Ionian mode scale"^^xsd:string ;
                        rdfs:label "has dominant chord in Ionian mode" .


###  http://example.org/fho/hasIonianLeadingtoneChord
:hasIonianLeadingtoneChord rdf:type owl:ObjectProperty ;
                           rdfs:subPropertyOf :hasLeadingtoneChord ;
                           rdfs:domain :IonianModeScale ;
                           rdfs:range mto:DiminishedTriad ;
                           rdfs:comment "Property to assign the chord with leadingtone degree to a Ionian mode scale"^^xsd:string ;
                           rdfs:label "has leadingtone chord in Ionian mode" .


###  http://example.org/fho/hasIonianMediantChord
:hasIonianMediantChord rdf:type owl:ObjectProperty ;
                       rdfs:subPropertyOf :hasMediantChord ;
                       rdfs:domain :IonianModeScale ;
                       rdfs:range mto:MinorTriad ;
                       rdfs:comment "Property to assign the chord with mediant degree to a Ionian mode scale"^^xsd:string ;
                       rdfs:label "has mediant chord in Ionian mode" .


###  http://example.org/fho/hasIonianSubdominantChord
:hasIonianSubdominantChord rdf:type owl:ObjectProperty ;
                           rdfs:subPropertyOf :hasSubdominantChord ;
                           rdfs:domain :IonianModeScale ;
                           rdfs:range mto:MajorTriad ;
                           rdfs:comment "Property to assign the chord with subdominant degree to a Ionian mode scale"^^xsd:string ;
                           rdfs:label "has subdominant chord in Ionian mode" .


###  http://example.org/fho/hasIonianSubmediantChord
:hasIonianSubmediantChord rdf:type owl:ObjectProperty ;
                          rdfs:subPropertyOf :hasSubmediantChord ;
                          rdfs:domain :IonianModeScale ;
                          rdfs:range mto:MinorTriad ;
                          rdfs:comment "Property to assign the chord with submediant degree to a Ionian mode scale"^^xsd:string ;
                          rdfs:label "has submediant chord in Ionian mode" .


###  http://example.org/fho/hasIonianSupertonicChord
:hasIonianSupertonicChord rdf:type owl:ObjectProperty ;
                          rdfs:subPropertyOf :hasSupertonicChord ;
                          rdfs:domain :IonianModeScale ;
                          rdfs:range mto:MinorTriad ;
                          rdfs:comment "Property to assign the chord with supertonic degree to a Ionian mode scale"^^xsd:string ;
                          rdfs:label "has supertonic chord in Ionian mode" .


###  http://example.org/fho/hasIonianTonicChord
:hasIonianTonicChord rdf:type owl:ObjectProperty ;
                     rdfs:subPropertyOf :hasTonicChord ;
                     rdfs:domain :IonianModeScale ;
                     rdfs:range mto:MajorTriad ;
                     rdfs:comment "Property to assign the chord with tonic degree to a Ionian mode scale"^^xsd:string ;
                     rdfs:label "has tonic chord in Ionian mode" .


###  http://example.org/fho/hasLeadingtoneChord
:hasLeadingtoneChord rdf:type owl:ObjectProperty ;
                     rdfs:subPropertyOf :hasChord ;
                     rdfs:domain mto:Scale ;
                     rdfs:range mto:Chord ;
                     owl:propertyChainAxiom ( :hasLeadingtoneNote
                                              [ owl:inverseOf chord:root
                                              ]
                                            ) ;
                     rdfs:comment "Property to assign the chord with leading degree degree to a scale"^^xsd:string ;
                     rdfs:label "has leading tone chord" .


###  http://example.org/fho/hasLeadingtoneNote
:hasLeadingtoneNote rdf:type owl:ObjectProperty ;
                    rdfs:subPropertyOf mto:hasNote ;
                    rdfs:domain mto:Scale ;
                    rdfs:range mto:Note ;
                    rdfs:comment "Property to assign the note with leading tone degree to a scale"^^xsd:string ;
                    rdfs:label "has leading tone note" .


###  http://example.org/fho/hasLocrianDominantChord
:hasLocrianDominantChord rdf:type owl:ObjectProperty ;
                         rdfs:subPropertyOf :hasDominantChord ;
                         rdfs:domain :LocrianModeScale ;
                         rdfs:range mto:MajorTriad ;
                         rdfs:comment "Property to assign the chord with dominant degree to a Locrian mode scale"^^xsd:string ;
                         rdfs:label "has dominant chord in Locrian mode" .


###  http://example.org/fho/hasLocrianLeadingtoneChord
:hasLocrianLeadingtoneChord rdf:type owl:ObjectProperty ;
                            rdfs:subPropertyOf :hasLeadingtoneChord ;
                            rdfs:domain :LocrianModeScale ;
                            rdfs:range mto:MinorTriad ;
                            rdfs:comment "Property to assign the chord with leadingtone degree to a Locrian mode scale"^^xsd:string ;
                            rdfs:label "has leadingtone chord in Locrian mode" .


###  http://example.org/fho/hasLocrianMediantChord
:hasLocrianMediantChord rdf:type owl:ObjectProperty ;
                        rdfs:subPropertyOf :hasMediantChord ;
                        rdfs:domain :LocrianModeScale ;
                        rdfs:range mto:MinorTriad ;
                        rdfs:comment "Property to assign the chord with mediant degree to a Locrian mode scale"^^xsd:string ;
                        rdfs:label "has mediant chord in Locrian mode" .


###  http://example.org/fho/hasLocrianSubdominantChord
:hasLocrianSubdominantChord rdf:type owl:ObjectProperty ;
                            rdfs:subPropertyOf :hasSubdominantChord ;
                            rdfs:domain :LocrianModeScale ;
                            rdfs:range mto:MinorTriad ;
                            rdfs:comment "Property to assign the chord with subdominant degree to a Locrian mode scale"^^xsd:string ;
                            rdfs:label "has subdominant chord in Locrian mode" .


###  http://example.org/fho/hasLocrianSubmediantChord
:hasLocrianSubmediantChord rdf:type owl:ObjectProperty ;
                           rdfs:subPropertyOf :hasSubmediantChord ;
                           rdfs:domain :LocrianModeScale ;
                           rdfs:range mto:MajorTriad ;
                           rdfs:comment "Property to assign the chord with submediant degree to a Locrian mode scale"^^xsd:string ;
                           rdfs:label "has submediant chord in Locrian mode" .


###  http://example.org/fho/hasLocrianSupertonicChord
:hasLocrianSupertonicChord rdf:type owl:ObjectProperty ;
                           rdfs:subPropertyOf :hasSupertonicChord ;
                           rdfs:domain :LocrianModeScale ;
                           rdfs:range mto:MajorTriad ;
                           rdfs:comment "Property to assign the chord with supertonic degree to a Locrian mode scale"^^xsd:string ;
                           rdfs:label "has supertonic chord in Locrian mode" .


###  http://example.org/fho/hasLocrianTonicChord
:hasLocrianTonicChord rdf:type owl:ObjectProperty ;
                      rdfs:subPropertyOf :hasTonicChord ;
                      rdfs:domain :LocrianModeScale ;
                      rdfs:range mto:DiminishedTriad ;
                      rdfs:comment "Property to assign the chord with tonic degree to a Locrian mode scale"^^xsd:string ;
                      rdfs:label "has tonic chord in Locrian mode" .


###  http://example.org/fho/hasLydianDominantChord
:hasLydianDominantChord rdf:type owl:ObjectProperty ;
                        rdfs:subPropertyOf :hasDominantChord ;
                        rdfs:domain :LydianModeScale ;
                        rdfs:range mto:MajorTriad ;
                        rdfs:comment "Property to assign the chord with dominant degree to a Lydian mode scale"^^xsd:string ;
                        rdfs:label "has dominant chord in Lydian mode" .


###  http://example.org/fho/hasLydianLeadingtoneChord
:hasLydianLeadingtoneChord rdf:type owl:ObjectProperty ;
                           rdfs:subPropertyOf :hasLeadingtoneChord ;
                           rdfs:domain :LydianModeScale ;
                           rdfs:range mto:MinorTriad ;
                           rdfs:comment "Property to assign the chord with leadingtone degree to a Lydian mode scale"^^xsd:string ;
                           rdfs:label "has leadingtone chord in Lydian mode" .


###  http://example.org/fho/hasLydianMediantChord
:hasLydianMediantChord rdf:type owl:ObjectProperty ;
                       rdfs:subPropertyOf :hasMediantChord ;
                       rdfs:domain :LydianModeScale ;
                       rdfs:range mto:MinorTriad ;
                       rdfs:comment "Property to assign the chord with mediant degree to a Lydian mode scale"^^xsd:string ;
                       rdfs:label "has mediant chord in Lydian mode" .


###  http://example.org/fho/hasLydianSubdominantChord
:hasLydianSubdominantChord rdf:type owl:ObjectProperty ;
                           rdfs:subPropertyOf :hasSubdominantChord ;
                           rdfs:domain :LydianModeScale ;
                           rdfs:range mto:DiminishedTriad ;
                           rdfs:comment "Property to assign the chord with subdominant degree to a Lydian mode scale"^^xsd:string ;
                           rdfs:label "has subdominant chord in Lydian mode" .


###  http://example.org/fho/hasLydianSubmediantChord
:hasLydianSubmediantChord rdf:type owl:ObjectProperty ;
                          rdfs:subPropertyOf :hasSubmediantChord ;
                          rdfs:domain :LydianModeScale ;
                          rdfs:range mto:MinorTriad ;
                          rdfs:comment "Property to assign the chord with submediant degree to a Lydian mode scale"^^xsd:string ;
                          rdfs:label "has submediant chord in Lydian mode" .


###  http://example.org/fho/hasLydianSupertonicChord
:hasLydianSupertonicChord rdf:type owl:ObjectProperty ;
                          rdfs:subPropertyOf :hasSupertonicChord ;
                          rdfs:domain :LydianModeScale ;
                          rdfs:range mto:MajorTriad ;
                          rdfs:comment "Property to assign the chord with supertonic degree to a Lydian mode scale"^^xsd:string ;
                          rdfs:label "has supertonic chord in Lydian mode" .


###  http://example.org/fho/hasLydianTonicChord
:hasLydianTonicChord rdf:type owl:ObjectProperty ;
                     rdfs:subPropertyOf :hasTonicChord ;
                     rdfs:domain :LydianModeScale ;
                     rdfs:range mto:MajorTriad ;
                     rdfs:comment "Property to assign the chord with tonic degree to a Lydian mode scale"^^xsd:string ;
                     rdfs:label "has tonic chord in Lydian mode" .


###  http://example.org/fho/hasMediantChord
:hasMediantChord rdf:type owl:ObjectProperty ;
                 rdfs:subPropertyOf :hasChord ;
                 rdfs:domain mto:Scale ;
                 rdfs:range mto:Chord ;
                 owl:propertyChainAxiom ( :hasMediantNote
                                          [ owl:inverseOf chord:root
                                          ]
                                        ) ;
                 rdfs:comment "Property to assign the chord with mediant degree to a scale"^^xsd:string ;
                 rdfs:label "has dominant chord" .


###  http://example.org/fho/hasMediantNote
:hasMediantNote rdf:type owl:ObjectProperty ;
                rdfs:subPropertyOf mto:hasNote ;
                rdfs:domain mto:Scale ;
                rdfs:range mto:Note ;
                rdfs:comment "Property to assign the note with mediant degree to a scale"^^xsd:string ;
                rdfs:label "has mediant note" .


###  http://example.org/fho/hasMixolydianDominantChord
:hasMixolydianDominantChord rdf:type owl:ObjectProperty ;
                            rdfs:subPropertyOf :hasDominantChord ;
                            rdfs:domain :MixolydianModeScale ;
                            rdfs:range mto:MinorTriad ;
                            rdfs:comment "Property to assign the chord with dominant degree to a Mixolydian mode scale"^^xsd:string ;
                            rdfs:label "has dominant chord in Mixolydian mode" .


###  http://example.org/fho/hasMixolydianLeadingtoneChord
:hasMixolydianLeadingtoneChord rdf:type owl:ObjectProperty ;
                               rdfs:subPropertyOf :hasLeadingtoneChord ;
                               rdfs:domain :MixolydianModeScale ;
                               rdfs:range mto:MajorTriad ;
                               rdfs:comment "Property to assign the chord with leadingtone degree to a Mixolydian mode scale"^^xsd:string ;
                               rdfs:label "has leadingtone chord in Mixolydian mode" .


###  http://example.org/fho/hasMixolydianMediantChord
:hasMixolydianMediantChord rdf:type owl:ObjectProperty ;
                           rdfs:subPropertyOf :hasMediantChord ;
                           rdfs:domain :MixolydianModeScale ;
                           rdfs:range mto:DiminishedTriad ;
                           rdfs:comment "Property to assign the chord with mediant degree to a Mixolydian mode scale"^^xsd:string ;
                           rdfs:label "has mediant chord in Mixolydian mode" .


###  http://example.org/fho/hasMixolydianSubdominantChord
:hasMixolydianSubdominantChord rdf:type owl:ObjectProperty ;
                               rdfs:subPropertyOf :hasSubdominantChord ;
                               rdfs:domain :MixolydianModeScale ;
                               rdfs:range mto:MajorTriad ;
                               rdfs:comment "Property to assign the chord with subdominant degree to a Mixolydian mode scale"^^xsd:string ;
                               rdfs:label "has subdominant chord in Mixolydian mode" .


###  http://example.org/fho/hasMixolydianSubmediantChord
:hasMixolydianSubmediantChord rdf:type owl:ObjectProperty ;
                              rdfs:subPropertyOf :hasSubmediantChord ;
                              rdfs:domain :MixolydianModeScale ;
                              rdfs:range mto:MinorTriad ;
                              rdfs:comment "Property to assign the chord with submediant degree to a Mixolydian mode scale"^^xsd:string ;
                              rdfs:label "has submediant chord in Mixolydian mode" .


###  http://example.org/fho/hasMixolydianSupertonicChord
:hasMixolydianSupertonicChord rdf:type owl:ObjectProperty ;
                              rdfs:subPropertyOf :hasSupertonicChord ;
                              rdfs:domain :MixolydianModeScale ;
                              rdfs:range mto:MinorTriad ;
                              rdfs:comment "Property to assign the chord with supertonic degree to a Mixolydian mode scale"^^xsd:string ;
                              rdfs:label "has supertonic chord in Mixolydian mode" .


###  http://example.org/fho/hasMixolydianTonicChord
:hasMixolydianTonicChord rdf:type owl:ObjectProperty ;
                         rdfs:subPropertyOf :hasTonicChord ;
                         rdfs:domain :MixolydianModeScale ;
                         rdfs:range mto:MajorTriad ;
                         rdfs:comment "Property to assign the chord with tonic degree to a Mixolydian mode scale"^^xsd:string ;
                         rdfs:label "has tonic chord in Mixolydian mode" .


###  http://example.org/fho/hasPhrygianDominantChord
:hasPhrygianDominantChord rdf:type owl:ObjectProperty ;
                          rdfs:subPropertyOf :hasDominantChord ;
                          rdfs:domain :PhrygianModeScale ;
                          rdfs:range mto:DiminishedTriad ;
                          rdfs:comment "Property to assign the chord with dominant degree to a Phrygian mode scale"^^xsd:string ;
                          rdfs:label "has dominant chord in Phrygian mode" .


###  http://example.org/fho/hasPhrygianLeadingtoneChord
:hasPhrygianLeadingtoneChord rdf:type owl:ObjectProperty ;
                             rdfs:subPropertyOf :hasLeadingtoneChord ;
                             rdfs:domain :PhrygianModeScale ;
                             rdfs:range mto:MinorTriad ;
                             rdfs:comment "Property to assign the chord with leadingtone degree to a Phrygian mode scale"^^xsd:string ;
                             rdfs:label "has leadingtone chord in Phrygian mode" .


###  http://example.org/fho/hasPhrygianMediantChord
:hasPhrygianMediantChord rdf:type owl:ObjectProperty ;
                         rdfs:subPropertyOf :hasMediantChord ;
                         rdfs:domain :PhrygianModeScale ;
                         rdfs:range mto:MajorTriad ;
                         rdfs:comment "Property to assign the chord with mediant degree to a Phrygian mode scale"^^xsd:string ;
                         rdfs:label "has mediant chord in Phrygian mode" .


###  http://example.org/fho/hasPhrygianSubdominantChord
:hasPhrygianSubdominantChord rdf:type owl:ObjectProperty ;
                             rdfs:subPropertyOf :hasSubdominantChord ;
                             rdfs:domain :PhrygianModeScale ;
                             rdfs:range mto:MinorTriad ;
                             rdfs:comment "Property to assign the chord with subdominant degree to a Phrygian mode scale"^^xsd:string ;
                             rdfs:label "has subdominant chord in Phrygian mode" .


###  http://example.org/fho/hasPhrygianSubmediantChord
:hasPhrygianSubmediantChord rdf:type owl:ObjectProperty ;
                            rdfs:subPropertyOf :hasSubmediantChord ;
                            rdfs:domain :PhrygianModeScale ;
                            rdfs:range mto:MajorTriad ;
                            rdfs:comment "Property to assign the chord with submediant degree to a Phrygian mode scale"^^xsd:string ;
                            rdfs:label "has submediant chord in Phrygian mode" .


###  http://example.org/fho/hasPhrygianSupertonicChord
:hasPhrygianSupertonicChord rdf:type owl:ObjectProperty ;
                            rdfs:subPropertyOf :hasSupertonicChord ;
                            rdfs:domain :PhrygianModeScale ;
                            rdfs:range mto:MajorTriad ;
                            rdfs:comment "Property to assign the chord with supertonic degree to a Phrygian mode scale"^^xsd:string ;
                            rdfs:label "has supertonic chord in Phrygian mode" .


###  http://example.org/fho/hasPhrygianTonicChord
:hasPhrygianTonicChord rdf:type owl:ObjectProperty ;
                       rdfs:subPropertyOf :hasTonicChord ;
                       rdfs:domain :PhrygianModeScale ;
                       rdfs:range mto:MinorTriad ;
                       rdfs:comment "Property to assign the chord with tonic degree to a Phrygian mode scale"^^xsd:string ;
                       rdfs:label "has tonic chord in Phrygian mode" .


###  http://example.org/fho/hasSubdominantChord
:hasSubdominantChord rdf:type owl:ObjectProperty ;
                     rdfs:subPropertyOf :hasChord ;
                     rdfs:domain mto:Scale ;
                     rdfs:range mto:Chord ;
                     owl:propertyChainAxiom ( :hasSubdominantNote
                                              [ owl:inverseOf chord:root
                                              ]
                                            ) ;
                     rdfs:comment "Property to assign the chord with subdominant degree to a scale"^^xsd:string ;
                     rdfs:label "has subdominant chord" .


###  http://example.org/fho/hasSubdominantNote
:hasSubdominantNote rdf:type owl:ObjectProperty ;
                    rdfs:subPropertyOf mto:hasNote ;
                    rdfs:domain mto:Scale ;
                    rdfs:range mto:Note ;
                    rdfs:comment "Property to assign the note with subdominant degree to a scale"^^xsd:string ;
                    rdfs:label "has subdominant note" .


###  http://example.org/fho/hasSubmediantChord
:hasSubmediantChord rdf:type owl:ObjectProperty ;
                    rdfs:subPropertyOf :hasChord ;
                    rdfs:domain mto:Scale ;
                    rdfs:range mto:Chord ;
                    owl:propertyChainAxiom ( :hasSubmediantNote
                                             [ owl:inverseOf chord:root
                                             ]
                                           ) ;
                    rdfs:comment "Property to assign the chord with submediant degree to a scale"^^xsd:string ;
                    rdfs:label "has submediant chord" .


###  http://example.org/fho/hasSubmediantNote
:hasSubmediantNote rdf:type owl:ObjectProperty ;
                   rdfs:subPropertyOf mto:hasNote ;
                   rdfs:domain mto:Scale ;
                   rdfs:range mto:Note ;
                   rdfs:comment "Property to assign the note with submediant degree to a scale"^^xsd:string ;
                   rdfs:label "has submediant note" .


###  http://example.org/fho/hasSupertonicChord
:hasSupertonicChord rdf:type owl:ObjectProperty ;
                    rdfs:subPropertyOf :hasChord ;
                    rdfs:domain mto:Scale ;
                    rdfs:range mto:Chord ;
                    owl:propertyChainAxiom ( :hasSupertonicNote
                                             [ owl:inverseOf chord:root
                                             ]
                                           ) ;
                    rdfs:comment "Property to assign the chord with supertonic degree to a scale"^^xsd:string ;
                    rdfs:label "has supertonic chord" .


###  http://example.org/fho/hasSupertonicNote
:hasSupertonicNote rdf:type owl:ObjectProperty ;
                   rdfs:subPropertyOf mto:hasNote ;
                   rdfs:domain mto:Scale ;
                   rdfs:range mto:Note ;
                   rdfs:comment "Property to assign the note with supertonic degree to a scale"^^xsd:string ;
                   rdfs:label "has supertonic note" .


###  http://example.org/fho/hasTonicChord
:hasTonicChord rdf:type owl:ObjectProperty ;
               rdfs:subPropertyOf :hasChord ;
               rdfs:domain mto:Scale ;
               rdfs:range mto:Chord ;
               owl:propertyChainAxiom ( :hasTonicNote
                                        [ owl:inverseOf chord:root
                                        ]
                                      ) ;
               rdfs:comment "Property to assign the chord with tonic degree to a scale"^^xsd:string ;
               rdfs:label "has tonic chord" .


###  http://example.org/fho/hasTonicNote
:hasTonicNote rdf:type owl:ObjectProperty ;
              rdfs:subPropertyOf mto:hasNote ;
              rdfs:domain mto:Scale ;
              rdfs:range mto:Note ;
              rdfs:comment "Property to assign the note with tonic degree to a scale"^^xsd:string ;
              rdfs:label "has tonic note" .


###  http://purl.org/ontology/chord/root
chord:root rdf:type owl:ObjectProperty .


###  http://purl.org/ontology/mto/hasNote
mto:hasNote rdf:type owl:ObjectProperty .


#################################################################
#    Classes
#################################################################

###  http://example.org/fho/AeolianModeScale
:AeolianModeScale rdf:type owl:Class ;
                  owl:equivalentClass mto:NaturalMinorScale ;
                  rdfs:subClassOf :ModeScale ;
                  rdfs:comment "Mode formed starting from the sixth degree of a major scale."^^xsd:string ;
                  rdfs:label "Aeolian Mode Scale"^^xsd:string .


###  http://example.org/fho/DorianModeScale
:DorianModeScale rdf:type owl:Class ;
                 rdfs:subClassOf :ModeScale ;
                 rdfs:comment "Mode formed starting from the second degree of a major scale."^^xsd:string ;
                 rdfs:label "Dorian Mode Scale"^^xsd:string .


###  http://example.org/fho/IonianModeScale
:IonianModeScale rdf:type owl:Class ;
                 owl:equivalentClass mto:MajorScale ;
                 rdfs:subClassOf :ModeScale ;
                 rdfs:comment "Mode formed starting from the first degree of a major scale."^^xsd:string ;
                 rdfs:label "Ionian Mode Scale"^^xsd:string .


###  http://example.org/fho/LocrianModeScale
:LocrianModeScale rdf:type owl:Class ;
                  rdfs:subClassOf :ModeScale ;
                  rdfs:comment "Mode formed starting from the seventh degree of a major scale."^^xsd:string ;
                  rdfs:label "Locrian Mode Scale"^^xsd:string .


###  http://example.org/fho/LydianModeScale
:LydianModeScale rdf:type owl:Class ;
                 rdfs:subClassOf :ModeScale ;
                 rdfs:comment "Mode formed starting from the fourth degree of a major scale."^^xsd:string ;
                 rdfs:label "Lydian Mode Scale"^^xsd:string .


###  http://example.org/fho/MixolydianModeScale
:MixolydianModeScale rdf:type owl:Class ;
                     rdfs:subClassOf :ModeScale ;
                     rdfs:comment "Mode formed starting from the fifth degree of a major scale."^^xsd:string ;
                     rdfs:label "Mixolydian Mode Scale"^^xsd:string .


###  http://example.org/fho/ModeScale
:ModeScale rdf:type owl:Class ;
           rdfs:subClassOf mto:HeptatonicScale ;
           rdfs:comment "A type of scale coupled with a set of characteristic melodic and harmonic behaviors defined by the root note of the scale." ;
           rdfs:label "Mode"^^xsd:string .


###  http://example.org/fho/PhrygianModeScale
:PhrygianModeScale rdf:type owl:Class ;
                   rdfs:subClassOf :ModeScale ;
                   rdfs:comment "Mode formed starting from the third degree of a major scale."^^xsd:string ;
                   rdfs:label "Phrygian Mode Scale"^^xsd:string .


###  http://purl.org/ontology/mto/Chord
mto:Chord rdf:type owl:Class .


###  http://purl.org/ontology/mto/DiminishedTriad
mto:DiminishedTriad rdf:type owl:Class .


###  http://purl.org/ontology/mto/HeptatonicScale
mto:HeptatonicScale rdf:type owl:Class .


###  http://purl.org/ontology/mto/MajorScale
mto:MajorScale rdf:type owl:Class .


###  http://purl.org/ontology/mto/MajorTriad
mto:MajorTriad rdf:type owl:Class .


###  http://purl.org/ontology/mto/MinorScale
mto:MinorScale rdf:type owl:Class .


###  http://purl.org/ontology/mto/MinorTriad
mto:MinorTriad rdf:type owl:Class .


###  http://purl.org/ontology/mto/NaturalMinorScale
mto:NaturalMinorScale rdf:type owl:Class .


###  http://purl.org/ontology/mto/Note
mto:Note rdf:type owl:Class .


###  http://purl.org/ontology/mto/Scale
mto:Scale rdf:type owl:Class .


###  Generated by the OWL API (version 4.5.9.2019-02-01T07:24:44Z) https://github.com/owlcs/owlapi
